src/proof/well_formed.v
@@ -3,97 +3,66 @@ From proof.k8s_io.api.apps Require Export v1_init.
 From proof.k8s_io.api.core Require Export v1_init.
 From proof.k8s_io.apimachinery.pkg.apis.meta Require Export v1_init.
 From proof Require Import prelude empty_ffi.
-From proof Require Export deepcopy.
+From proof Require Export deepown.
 
 
 Section proof.
 Context `{hG: !heapGS Σ} {go_ctx: GoContext}.
 
-Definition has_controller_parent l os i o c : iProp Σ :=
-  l ↦*□ os ∗ ⌜ os !! i = Some o ⌝ ∗ o.(v1.OwnerReference.Controller') ↦□ c ∗ ⌜ c = true ⌝.
+(* https://github.com/kubernetes/kubernetes/blob/release-1.34/staging/src/k8s.io/apimachinery/pkg/api/validation/objectmeta.go#L169 *)
+Axiom valid_name: go_string → Prop.
 
-Definition has_controller_parent_of l uid : iProp Σ :=
-  ∃ os i o c, has_controller_parent l os i o c ∗ ⌜ o.(v1.OwnerReference.UID') = uid ⌝.
+(* https://github.com/kubernetes/kubernetes/blob/release-1.34/staging/src/k8s.io/apimachinery/pkg/api/validation/objectmeta.go#L177 *)
+Axiom valid_namespace: go_string → Prop.
 
-Definition has_controller_parent_at l i : iProp Σ :=
-  ∃ os o c, has_controller_parent l os i o c.
-
-Definition well_formed_OwnerReferences l : iProp Σ :=
+Definition well_formed_OwnerReferences (os: list PureOwnerReference.t) : Prop :=
   (* https://github.com/kubernetes/kubernetes/blob/release-1.34/staging/src/k8s.io/apimachinery/pkg/api/validation/objectmeta.go#L92 *)
-  "#at_most_one_controller_parent" ∷ □ ∀ i1 i2,
-    has_controller_parent_at l i1 -∗ has_controller_parent_at l i2 -∗ ⌜ i1 = i2 ⌝.
+  ∀ i1 o1 i2 o2,
+    os !! i1 = Some o1 ∧ o1.(PureOwnerReference.Controller') = Some true ∧
+    os !! i2 = Some o2 ∧ o2.(PureOwnerReference.Controller') = Some true →
+      i1 = i2.
 
-Definition well_formed_ObjectMeta (m: v1.ObjectMeta.t) : iProp Σ :=
-  "%uid_well_formed" ∷ ⌜ m.(v1.ObjectMeta.UID') ≠ "_ORPHAN_POD"%go ⌝ ∗
-  "#well_formed_OwnerReferences" ∷ well_formed_OwnerReferences m.(v1.ObjectMeta.OwnerReferences').
+(* TODO: translate https://github.com/kubernetes/kubernetes/blob/release-1.34/staging/src/k8s.io/apimachinery/pkg/api/validation/objectmeta.go to spec *)
+Definition well_formed_ObjectMeta (m: PureObjectMeta.t) : Prop :=
+  (m.(PureObjectMeta.GenerateName') ≠ ""%go → valid_name m.(PureObjectMeta.GenerateName')) ∧
+  m.(PureObjectMeta.Name') ≠ ""%go ∧
+  valid_name m.(PureObjectMeta.Name') ∧
+  m.(PureObjectMeta.Namespace') ≠ ""%go ∧
+  valid_namespace m.(PureObjectMeta.Namespace') ∧
+  match m.(PureObjectMeta.OwnerReferences') with
+  | None => True
+  | Some os => well_formed_OwnerReferences os
+  end.
 
-Lemma at_most_one_controller_parent_implies_same_uid o:
-  (□ ∀ i1 i2, has_controller_parent_at o i1 -∗ has_controller_parent_at o i2 -∗ ⌜ i1 = i2 ⌝)
-  ⊢ (□ ∀ uid1 uid2, has_controller_parent_of o uid1 -∗ has_controller_parent_of o uid2 -∗ ⌜ uid1 = uid2 ⌝).
-Proof.
-  iIntros "#H". iModIntro.
-  iIntros (uid1 uid2) "Huid1 Huid2".
-  iDestruct "Huid1" as (os1 i1 o1 c1) "[Hparent1 %Huid1]".
-  iDestruct "Huid2" as (os2 i2 o2 c2) "[Hparent2 %Huid2]".
-  iDestruct ("H" $! i1 i2 with "[Hparent1] [Hparent2]") as "%Hi_eq".
-  { iExists os1, o1, c1. iFrame "Hparent1". }
-  { iExists os2, o2, c2. iFrame "Hparent2". }
-  subst i2.
-  iDestruct "Hparent1" as "(#Hos1 & %Hlookup1 & _)".
-  iDestruct "Hparent2" as "(#Hos2 & %Hlookup2 & _)".
-  iDestruct (own_slice_agree with "Hos1 Hos2") as %Hos_eq.
-  subst os2.
-  rewrite Hlookup1 in Hlookup2.
-  injection Hlookup2 as <-.
-  iPureIntro.
-  congruence.
-Qed.
+Axiom well_formed_PodSpec: PurePodSpec.t → Prop.
 
-Axiom well_formed_PodSpec: v1.PodSpec.t → iProp Σ.
-Global Instance well_formed_PodSpec_persistent spec : Persistent (well_formed_PodSpec spec).
-Proof. Admitted.
+Axiom well_formed_PodStatus: PurePodStatus.t → Prop.
 
-Axiom well_formed_PodStatus: v1.PodStatus.t → iProp Σ.
-Global Instance well_formed_PodStatus_persistent status : Persistent (well_formed_PodStatus status).
-Proof. Admitted.
+Definition well_formed_Pod (pod: PurePod.t) : Prop :=
+  well_formed_ObjectMeta pod.(PurePod.ObjectMeta') ∧
+  well_formed_PodSpec pod.(PurePod.Spec') ∧
+  well_formed_PodStatus pod.(PurePod.Status').
 
-Definition well_formed_Pod (pod: v1.Pod.t) : iProp Σ :=
-  "#pod_metadata_well_formed" ∷ well_formed_ObjectMeta pod.(v1.Pod.ObjectMeta') ∗
-  "#well_formed_PodSpec" ∷ well_formed_PodSpec pod.(v1.Pod.Spec') ∗
-  "#well_formed_PodStatus" ∷ well_formed_PodStatus pod.(v1.Pod.Status').
+Definition well_formed_to_create_ObjectMeta (m: PureObjectMeta.t) : Prop :=
+  (m.(PureObjectMeta.Name') = ""%go → m.(PureObjectMeta.GenerateName') ≠ ""%go) ∧
+  match m.(PureObjectMeta.OwnerReferences') with
+  | None => True
+  | Some os => well_formed_OwnerReferences os
+  end.
 
-Definition well_formed_to_create_ObjectMeta (m: v1.ObjectMeta.t) : iProp Σ :=
-  "%generatename_not_empty_if_name_empty" ∷ ⌜ m.(v1.ObjectMeta.Name') = ""%go → m.(v1.ObjectMeta.GenerateName') ≠ ""%go ⌝.
+(* Axiom well_formed_to_create_PodSpec: PurePodSpec.t → Prop.
 
-Axiom well_formed_to_create_PodSpec: v1.PodSpec.t → iProp Σ.
-Global Instance well_formed_to_create_PodSpec_persistent spec : Persistent (well_formed_to_create_PodSpec spec).
-Proof. Admitted.
+Axiom well_formed_to_create_PodStatus: PurePodStatus.t → Prop. *)
 
-Axiom well_formed_to_create_PodStatus: v1.PodStatus.t → iProp Σ.
-Global Instance well_formed_to_create_PodStatus_persistent status : Persistent (well_formed_to_create_PodStatus status).
-Proof. Admitted.
+Definition well_formed_to_create_Pod (pod: PurePod.t) : Prop :=
+  well_formed_to_create_ObjectMeta pod.(PurePod.ObjectMeta') ∧
+  well_formed_PodSpec pod.(PurePod.Spec') ∧
+  well_formed_PodStatus pod.(PurePod.Status').
+  (* well_formed_to_create_PodSpec pod.(PurePod.Spec') ∧ *)
+  (* well_formed_to_create_PodStatus pod.(PurePod.Status'). *)
 
-Definition well_formed_to_create_Pod (pod: v1.Pod.t) : iProp Σ :=
-  "#pod_metadata_to_create_well_formed" ∷ well_formed_to_create_ObjectMeta pod.(v1.Pod.ObjectMeta') ∗
-  "#well_formed_to_create_PodSpec" ∷ well_formed_to_create_PodSpec pod.(v1.Pod.Spec') ∗
-  "#well_formed_to_create_PodStatus" ∷ well_formed_to_create_PodStatus pod.(v1.Pod.Status').
-
-Definition well_formed_ReplicaSet (rs: v1.ReplicaSet.t) : iProp Σ :=
-  well_formed_ObjectMeta rs.(v1.ReplicaSet.ObjectMeta') ∗
-  ∃ (v: w32), rs.(v1.ReplicaSet.Spec').(v1.ReplicaSetSpec.Replicas') ↦□ v ∗ ⌜ 0 ≤ sint.Z v ⌝.
-
-Lemma well_formed_preserved_by_deepcopy_ReplicaSet rs1 rs2 namespace name:
-  deepcopy_ReplicaSet rs1 rs2 -∗
-    ⌜ rs1.(v1.ReplicaSet.ObjectMeta').(v1.ObjectMeta.Namespace') = namespace ⌝ -∗
-    ⌜ rs1.(v1.ReplicaSet.ObjectMeta').(v1.ObjectMeta.Name') = name ⌝ -∗
-    well_formed_ReplicaSet rs1 -∗
-      deepcopy_ReplicaSet rs1 rs2 ∗
-      ⌜ rs1.(v1.ReplicaSet.ObjectMeta').(v1.ObjectMeta.Namespace') = namespace ⌝ ∗
-      ⌜ rs1.(v1.ReplicaSet.ObjectMeta').(v1.ObjectMeta.Name') = name ⌝ ∗
-      ⌜ rs2.(v1.ReplicaSet.ObjectMeta').(v1.ObjectMeta.Namespace') = namespace ⌝ ∗
-      ⌜ rs2.(v1.ReplicaSet.ObjectMeta').(v1.ObjectMeta.Name') = name ⌝ ∗
-      well_formed_ReplicaSet rs2.
-Proof.
-Admitted.
+Definition well_formed_ReplicaSet (rs: PureReplicaSet.t) : Prop :=
+  well_formed_ObjectMeta rs.(PureReplicaSet.ObjectMeta') ∧
+  (∃ (v: w32), rs.(PureReplicaSet.Spec').(PureReplicaSetSpec.Replicas') = Some v ∧ 0 ≤ sint.Z v).
 
 End proof.
